ia32/Asm.v
@@ -915,7 +915,7 @@ Inductive step: state -> trace -> state -> Prop :=
       Genv.find_funct_ptr ge b = Some (External ef) ->
       extcall_arguments rs m (ef_sig ef) args ->
       external_call ef (fun _ => True) ge args m t res m' ->
-      rs' = (set_pair (loc_external_result (ef_sig ef)) res rs) #PC <- (rs RA) ->
+      rs' = (set_pair (loc_external_result (ef_sig ef)) res rs) #PC <- (rs RA) #RA <- Vundef ->
       step (State rs m) t (State rs' m').
 
 End RELSEM.
