ia32/Asmgenproof.v
@@ -353,6 +353,10 @@ Qed.
 - Mach register values and PPC register values agree.
 *)
 
+Section WITHINITSPRA.
+
+Variables init_sp init_ra: val.
+
 Inductive match_states: Mach.state -> Asm.state -> Prop :=
   | match_states_intro:
       forall s fb sp c ep ms m m' rs f tf tc
@@ -361,24 +365,25 @@ Inductive match_states: Mach.state -> Asm.state -> Prop :=
         (MEXT: Mem.extends m m')
         (AT: transl_code_at_pc ge (rs PC) fb f c ep tf tc)
         (AG: agree ms sp rs)
-        (DXP: ep = true -> rs#EDX = parent_sp s),
+        (DXP: ep = true -> rs#EDX = parent_sp init_sp s),
       match_states (Mach.State s fb sp c ms m)
                    (Asm.State rs m')
   | match_states_call:
       forall s fb ms m m' rs
         (STACKS: match_stack ge s)
         (MEXT: Mem.extends m m')
-        (AG: agree ms (parent_sp s) rs)
+        (AG: agree ms (parent_sp init_sp s) rs)
         (ATPC: rs PC = Vptr fb Int.zero)
-        (ATLR: rs RA = parent_ra s),
+        (ATLR: rs RA = parent_ra init_ra s),
       match_states (Mach.Callstate s fb ms m)
                    (Asm.State rs m')
   | match_states_return:
       forall s ms m m' rs
         (STACKS: match_stack ge s)
         (MEXT: Mem.extends m m')
-        (AG: agree ms (parent_sp s) rs)
-        (ATPC: rs PC = parent_ra s),
+        (AG: agree ms (parent_sp init_sp s) rs)
+        (RA_VUNDEF: rs RA = Vundef)
+        (ATPC: rs PC = parent_ra init_ra s),
       match_states (Mach.Returnstate s ms m)
                    (Asm.State rs m').
 
@@ -392,7 +397,7 @@ Lemma exec_straight_steps:
    exists rs2,
        exec_straight tge tf c rs1 m1' k rs2 m2'
     /\ agree ms2 sp rs2
-    /\ (it1_is_parent ep i = true -> rs2#EDX = parent_sp s)) ->
+    /\ (it1_is_parent ep i = true -> rs2#EDX = parent_sp init_sp s)) ->
   exists st',
   plus step tge (State rs1 m1') E0 st' /\
   match_states (Mach.State s fb sp c ms2 m2) st'.
@@ -458,8 +463,11 @@ Definition measure (s: Mach.state) : nat :=
 
 (** This is the simulation diagram.  We prove it by case analysis on the Mach transition. *)
 
+Hypothesis init_sp_not_vundef: init_sp <> Vundef.
+Hypothesis init_ra_not_vundef: init_ra <> Vundef.
+
 Theorem step_simulation:
-  forall S1 t S2, Mach.step return_address_offset ge S1 t S2 ->
+  forall S1 t S2, Mach.step init_sp init_ra return_address_offset ge S1 t S2 ->
   forall S1' (MS: match_states S1 S1'),
   (exists S2', plus step tge S1' t S2' /\ match_states S2 S2')
   \/ (measure S2 < measure S1 /\ t = E0 /\ match_states S2 S1')%nat.
@@ -499,7 +507,7 @@ Local Transparent destroyed_by_setstack.
   unfold load_stack in *.
   exploit Mem.loadv_extends. eauto. eexact H0. auto.
   intros [parent' [A B]]. rewrite (sp_val _ _ _ AG) in A.
-  exploit lessdef_parent_sp; eauto. clear B; intros B; subst parent'.
+  exploit (lessdef_parent_sp init_sp); eauto. clear B; intros B; subst parent'.
   exploit Mem.loadv_extends. eauto. eexact H1. auto.
   intros [v' [C D]].
 Opaque loadind.
@@ -611,8 +619,8 @@ Opaque loadind.
   rewrite (sp_val _ _ _ AG) in *. unfold load_stack in *.
   exploit Mem.loadv_extends. eauto. eexact H1. auto. simpl. intros [parent' [A B]].
   exploit Mem.loadv_extends. eauto. eexact H2. auto. simpl. intros [ra' [C D]].
-  exploit lessdef_parent_sp; eauto. intros. subst parent'. clear B.
-  exploit lessdef_parent_ra; eauto. intros. subst ra'. clear D.
+  exploit (lessdef_parent_sp init_sp); eauto. intros. subst parent'. clear B.
+  exploit (lessdef_parent_ra init_ra); eauto. intros. subst ra'. clear D.
   exploit Mem.free_parallel_extends; eauto. intros [m2' [E F]].
   destruct ros as [rf|fid]; simpl in H; monadInv H7.
 + (* Indirect call *)
@@ -789,9 +797,9 @@ Transparent destroyed_by_jumptable.
     eapply transf_function_no_overflow; eauto.
   rewrite (sp_val _ _ _ AG) in *. unfold load_stack in *.
   exploit Mem.loadv_extends. eauto. eexact H0. auto. simpl. intros [parent' [A B]].
-  exploit lessdef_parent_sp; eauto. intros. subst parent'. clear B.
+  exploit (lessdef_parent_sp init_sp); eauto. intros. subst parent'. clear B.
   exploit Mem.loadv_extends. eauto. eexact H1. auto. simpl. intros [ra' [C D]].
-  exploit lessdef_parent_ra; eauto. intros. subst ra'. clear D.
+  exploit (lessdef_parent_ra init_ra); eauto. intros. subst ra'. clear D.
   exploit Mem.free_parallel_extends; eauto. intros [m2' [E F]].
   monadInv H6.
   exploit code_tail_next_int; eauto. intro CT1.
@@ -849,6 +857,7 @@ Transparent destroyed_at_function_entry.
   eapply external_call_symbols_preserved; eauto. apply senv_preserved.
   econstructor; eauto.
   unfold loc_external_result.
+  apply agree_set_other; auto.
   apply agree_set_other; auto. apply agree_set_pair; auto.
 
 - (* return *)
@@ -857,9 +866,11 @@ Transparent destroyed_at_function_entry.
   econstructor; eauto. rewrite ATPC; eauto. congruence.
 Qed.
 
+End WITHINITSPRA.
+
 Lemma transf_initial_states:
   forall st1, Mach.initial_state prog st1 ->
-  exists st2, Asm.initial_state tprog st2 /\ match_states st1 st2.
+  exists st2, Asm.initial_state tprog st2 /\ match_states Vzero Vzero st1 st2.
 Proof.
   intros. inversion H. unfold ge0 in *.
   econstructor; split.
@@ -879,7 +890,7 @@ Qed.
 
 Lemma transf_final_states:
   forall st1 st2 r,
-  match_states st1 st2 -> Mach.final_state st1 r -> Asm.final_state st2 r.
+  match_states Vzero Vzero st1 st2 -> Mach.final_state st1 r -> Asm.final_state st2 r.
 Proof.
   intros. inv H0. inv H. constructor. auto.
   compute in H1. inv H1.
@@ -893,7 +904,7 @@ Proof.
   apply senv_preserved.
   eexact transf_initial_states.
   eexact transf_final_states.
-  exact step_simulation.
+  apply step_simulation; unfold Vzero; congruence.
 Qed.
 
 End PRESERVATION.
