backend/CleanupLabelsproof.v
@@ -229,9 +229,10 @@ Definition measure (st: state) : nat :=
   end.
 
 Lemma match_parent_locset:
+  forall init_ls,
   forall s ts,
   list_forall2 match_stackframes s ts ->
-  parent_locset ts = parent_locset s.
+  parent_locset init_ls ts = parent_locset init_ls s.
 Proof.
   induction 1; simpl. auto. inv H; auto.
 Qed.
@@ -240,10 +241,12 @@ Qed.
 Section WITHWRITABLEBLOCK.
 Context `{Hwritable_block: WritableBlock}.
 
+Variable init_ls: locset.
+
 Theorem transf_step_correct:
-  forall s1 t s2, step ge s1 t s2 ->
+  forall s1 t s2, step init_ls ge s1 t s2 ->
   forall s1' (MS: match_states s1 s1'),
-  (exists s2', step tge s1' t s2' /\ match_states s2 s2')
+  (exists s2', step init_ls tge s1' t s2' /\ match_states s2 s2')
   \/ (measure s2 < measure s1 /\ t = E0 /\ match_states s2 s1')%nat.
 Proof.
   induction 1; intros; inv MS; try rewrite remove_unused_labels_cons.
@@ -376,7 +379,7 @@ Proof.
   apply senv_preserved.
   eexact transf_initial_states.
   eexact transf_final_states.
-  eexact transf_step_correct.
+  apply transf_step_correct.
 Qed.
 
 End CLEANUP.
