backend/Tunnelingproof.v
@@ -270,18 +270,20 @@ Definition measure (st: state) : nat :=
 Section WITHWRITABLEBLOCK.
 Context `{Hwritable_block: WritableBlock}.
 
+Variable init_ls: locset.
+
 Lemma match_parent_locset:
   forall s ts,
   list_forall2 match_stackframes s ts ->
-  parent_locset ts = parent_locset s.
+  parent_locset init_ls ts = parent_locset init_ls s.
 Proof.
   induction 1; simpl. auto. inv H; auto.
 Qed.
 
 Lemma tunnel_step_correct:
-  forall st1 t st2, step ge st1 t st2 ->
+  forall st1 t st2, step init_ls ge st1 t st2 ->
   forall st1' (MS: match_states st1 st1'),
-  (exists st2', step tge st1' t st2' /\ match_states st2 st2')
+  (exists st2', step init_ls tge st1' t st2' /\ match_states st2 st2')
   \/ (measure st2 < measure st1 /\ t = E0 /\ match_states st2 st1')%nat.
 Proof.
   induction 1; intros; try inv MS.
@@ -289,7 +291,7 @@ Proof.
   (* entering a block *)
   assert (DEFAULT: branch_target f pc = pc ->
     (exists st2' : state,
-     step tge (State ts (tunnel_function f) sp (branch_target f pc) rs m) E0 st2'
+     step init_ls tge (State ts (tunnel_function f) sp (branch_target f pc) rs m) E0 st2'
      /\ match_states (Block s f sp bb rs m) st2')).
   intros. rewrite H0. econstructor; split.
   econstructor. simpl. rewrite PTree.gmap1. rewrite H. simpl. eauto.
@@ -429,7 +431,7 @@ Proof.
   apply senv_preserved.
   eexact transf_initial_states.
   eexact transf_final_states.
-  eexact tunnel_step_correct.
+  apply tunnel_step_correct.
 Qed.
 
 End PRESERVATION.
